# Review

## Tuples

### Syntax

```haskell
t = (1, 2)
fst t -- returns 1
snd t -- returns 2
```

## Types

Haskell compiler does two things:

1. Type checking: check if the usage of explicit types is valid.
2. Type inference: converts implicit types to explicit types.

### Exercise

Try to understand what the code below is doing and try to check its type:

~~~haskell
import Data.Function (on)
import Data.List (sortBy)

sortBy (compare `on` fst)
		[(2 :: Int,"Albert"), (1,"David"), (3,"AsbjÃ¸rn")]
~~~

Syntax sugar:

~~~haskell 
1 `+` 2 == (+) 1 2
~~~


#### Checking the types of the functions:

```
 sortBy :: (a0 -> a0 -> Ordering) -> [a0] -> [a0]
compare :: Ord a1 => a1 -> a1 -> Ordering
     on :: (b1 -> b1 -> c) -> (a2 -> b1) -> a2 -> a2 -> c
    fst :: (a3, b2) -> a3
```

on compare fst
Hence:

- Based on `sortBy`

	a0 => (Int, String)	

- Based on `fst`

	a3 => Int
	
	b2 => String	


- Base on `on`
	
	(b1 -> b1 -> c) is (a1 -> a1 -> Ordering)
	
	(a2 -> b1) is ((a3, b2) -> a3)
	
	That is 
	
	a2 => (Int, String)
	
	b1 => Int
	
	a1 => Int
	
	c => Ordering

Conclusion:

```haskell
a0 :: (Int, String)
a1 :: Int
a2 :: (Int, String)
a3 :: Int
b1 :: Int
b2 :: String
c  :: Ordering
```


# Unfold, Map, Fold

## Unfold

A generator that will produce sequence of values based on some initial value.

### Example

```haskell
import Data.List (unfoldr)

unfoldr :: (b -> Maybe (a, b)) -> b -> [a]
```

A value with `Maybe` type is either:

1. Nothing 
2. Just

> This is exactly the optional in Swift.


--

Generate `[1..10]` using `unfoldr`:

```haskell
unfoldr(\e -> if e > 10 then Nothing else Just(e, e + 1)) 1
```

The second element in the `Just` tuple will be passed to the next iteration.
 
--

Generate `[1..]` using `unfoldr`:

```haskell
unfoldr(\e -> Just(e, e+1)) 1
```

### Exercise

1. Define `repeat` using `unfoldr`:

	```haskell
	repeat' :: a -> [a]
	repeat' element = unfoldr(\e -> Just(e, e)) element
	```

2. Define `iterate` using `unfoldr`:

	```haskell
	iterate' :: (a -> a) -> a -> [a]
	iterate' mapper element = unfoldr(\e -> Just(e, mapper(e))) element
	```

3. Define `take` using `unfoldr`:

	*Bad implementation*:
	
	```haskell
	take' :: Int -> [a] -> [a]
	take' count list = unfoldr(\e -> if length list - length e < count 
		then Just(head e, tail e) 
		else Nothing) list
	```

	Check the number of taken elements by comparing the difference of the length of complete list and current list.
	
	This may cause some problem when the length of the list cannot be determined.
	
	*Better implementation*:
	
	```haskell
	take' :: Int -> [a] -> [a]
	take' count list = unfoldr g (count, list) 
		where g (count, list) = if count > 0
			then Just(head list, (count - 1, tail list))
			else Nothing
	``` 
	
	Idea: pass remaining count with current list into `unfoldr`.
	

## Fold

A collector that will collect values in a list into a single value (a.k.a. `reduce`).

### Example

There are 2 kinds of `fold` in Haskell:

1. `foldl`: starts from the **first** element.
	
	```haskell
	foldl :: Foldable t => (b -> a -> b) -> b -> t a -> b
	
	-- take each element and append at the end
	foldl(\mem ele -> mem ++ [ele]) [] [1, 2, 3]
	```
	
	Output:
	
	```haskell
	[1, 2, 3]
	```
	
2. `foldr`: starts from the **last** element.

	```haskell
	foldr :: Foldable t => (a -> b -> b) -> b -> t a -> b
	
	-- take each element and append at the end
	foldr(\ele mem -> mem ++ [ele]) [] [1, 2, 3]
	```
	
	Output:
	
	```haskell
	[3, 2, 1]
	```

--

Define `and` using `foldr` / `foldl`:

```haskell
and' :: Foldable t => t Bool -> Bool

-- using foldr
and' list = foldr(\ele mem -> ele && mem) True list

-- using foldl
and' list = foldl(\mem ele -> ele && mem) True list
```

Define `sum` using `foldr` / `foldl`:

```haskell
sum' :: (Num a, Foldable t) => t a -> a

-- using foldr
sum' list = foldr(\ele mem -> ele + mem) 0 list

-- using foldl
sum' list = foldl(\mem ele -> ele + mem) 0 list
```

Define `concat` using `foldr` / `foldl`:

```haskell
concat' :: Foldable t => t [a] -> [a]

-- using foldr
concat' list = foldr(\ele mem -> ele ++ mem) [] list

-- using foldl
concat' list = foldl(\mem ele -> mem ++ ele) [] list
```

Find the `max` element of a list using `foldr` / `foldl`:

```haskell
lmax :: (Ord a,  Foldable t) => t [a] -> a

lmax list = foldl(\mem ele -> if ele > mem 
	then ele 
	else mem) (head list) list

```

### Exercise

1. Define `length` using `foldr` / `foldl`:

	```haskell
	length' :: [a] -> Int

	length' list = foldl(\mem _ -> mem + 1) 0 list
	```
	
	Underscore(`_`) denotes the unused variable (can be ignored).
	
2. Define `reverse` using `foldr` / `foldl`:

	```haskell
	reverse' :: [a] -> [a]
	
	-- use foldl
	reverse' list = foldl(\mem ele -> ele : mem) [] list
	
	-- or use foldr
	reverse' list = foldr(\ele mem -> mem ++ [ele]) [] list
	```

3. Define `zipWith` using `foldr` / `foldl`:

	```haskell
	zipWith' :: (a -> b -> c) -> [a] -> [b] -> [c]
	
	zipWith' mapper list1 list2 = snd $ foldl g (list1, []) list2 
		where g (list1, result) e = (tail list1, result ++ [mapper (head list1) e])
	```
	
	Idea: 
	- We need to remove `head` from `list1` when `list2` advances. 
	- Make the `memory` object a tuple and put the `result` and the `list1` in that tuple.
	- Update the tuple in each iteration (replace `list1` as `tail list1`).


## Map

Convert each of the elements in a list into other values and put the new value in a new list.

### Example

Define `filter` using `map`:

```haskell
filter' :: (a -> Bool) -> [a] -> [a]
filter' condition list = concat $ map(\e -> if condition e 
	then [e] 
	else []) list
```

Define `length` using `map`:

```haskell
length' :: [a] -> Int
length' list = sum $ map(const 1) list
```

### Exercise

1. Check if a sequence is a palindrome:
	
	```haskell
	palindrome :: Eq a => [a] -> Bool
	
	palindrome list = and $ zipWith(\a b -> a == b) list (reverse list)
	
	-- or 
	
	palindrome list = list == reverse(list)
	```

2. Define `map` using `foldr` / `foldl`:

	```haskell 
	map' :: (a -> b) -> [a] -> [b]
	
	map' mapper list = foldl(\mem ele -> mem ++ [mapper ele]) [] list
	```